CollapsingTowers/TwoLevel/OpenClose.lean
@@ -6,8 +6,8 @@ import Mathlib.Data.Finset.Max
 def fv : Expr → Finset ℕ
   | .bvar _ => ∅
   | .fvar y => { y }
-  | .lam₁ _ e => fv e
-  | .lam₂ _ e => fv e
+  | .lam₁ e => fv e
+  | .lam₂ e => fv e
   | .app₁ f arg => fv f ∪ fv arg
   | .app₂ f arg => fv f ∪ fv arg
   | .lit₁ _ => ∅
@@ -16,7 +16,7 @@ def fv : Expr → Finset ℕ
   | .plus₂ l r => fv l ∪ fv r
   | .code e => fv e
   | .reflect e => fv e
-  | .lam𝕔 _ e => fv e
+  | .lam𝕔 e => fv e
   | .lets b e => fv b ∪ fv e
   | .let𝕔 b e => fv b ∪ fv e
 
@@ -28,8 +28,8 @@ def fresh (e : Expr) : ℕ :=
 def subst (x : ℕ) (v : Expr) : Expr -> Expr
   | .bvar i => .bvar i
   | .fvar y => if x = y then v else .fvar y
-  | .lam₁ τ e => .lam₁ τ (subst x v e)
-  | .lam₂ τ e => .lam₂ τ (subst x v e)
+  | .lam₁ e => .lam₁ (subst x v e)
+  | .lam₂ e => .lam₂ (subst x v e)
   | .app₁ f arg => .app₁ (subst x v f) (subst x v arg)
   | .app₂ f arg => .app₂ (subst x v f) (subst x v arg)
   | .lit₁ n => .lit₁ n
@@ -38,7 +38,7 @@ def subst (x : ℕ) (v : Expr) : Expr -> Expr
   | .plus₂ l r => .plus₂ (subst x v l) (subst x v r)
   | .code e => .code (subst x v e)
   | .reflect e => .reflect (subst x v e)
-  | .lam𝕔 τ e => .lam𝕔 τ (subst x v e)
+  | .lam𝕔 e => .lam𝕔 (subst x v e)
   | .lets b e => .lets (subst x v b) (subst x v e)
   | .let𝕔 b e => .let𝕔 (subst x v b) (subst x v e)
 
@@ -47,8 +47,8 @@ def subst (x : ℕ) (v : Expr) : Expr -> Expr
 def opening (i : ℕ) (x : Expr) : Expr -> Expr
   | .bvar j => if j = i then x else .bvar j
   | .fvar x => .fvar x
-  | .lam₁ τ e => .lam₁ τ (opening (i + 1) x e)
-  | .lam₂ τ e => .lam₂ τ (opening (i + 1) x e)
+  | .lam₁ e => .lam₁ (opening (i + 1) x e)
+  | .lam₂ e => .lam₂ (opening (i + 1) x e)
   | .app₁ f arg => .app₁ (opening i x f) (opening i x arg)
   | .app₂ f arg => .app₂ (opening i x f) (opening i x arg)
   | .lit₁ n => .lit₁ n
@@ -57,7 +57,7 @@ def opening (i : ℕ) (x : Expr) : Expr -> Expr
   | .plus₂ l r => .plus₂ (opening i x l) (opening i x r)
   | .code e => .code (opening i x e)
   | .reflect e => .reflect (opening i x e)
-  | .lam𝕔 τ e => .lam𝕔 τ (opening (i + 1) x e)
+  | .lam𝕔 e => .lam𝕔 (opening (i + 1) x e)
   | .lets b e => .lets (opening i x b) (opening (i + 1) x e)
   | .let𝕔 b e => .let𝕔 (opening i x b) (opening (i + 1) x e)
 
@@ -73,8 +73,8 @@ def open_subst (tgt : Expr) (within : Expr) :=
 def closing (i : ℕ) (x : ℕ) : Expr -> Expr
   | .bvar j => .bvar j
   | .fvar y => if x == y then .bvar i else .fvar y
-  | .lam₁ τ e => .lam₁ τ (closing (i + 1) x e)
-  | .lam₂ τ e => .lam₂ τ (closing (i + 1) x e)
+  | .lam₁ e => .lam₁ (closing (i + 1) x e)
+  | .lam₂ e => .lam₂ (closing (i + 1) x e)
   | .app₁ f arg => .app₁ (closing i x f) (closing i x arg)
   | .app₂ f arg => .app₂ (closing i x f) (closing i x arg)
   | .lit₁ n => .lit₁ n
@@ -83,7 +83,7 @@ def closing (i : ℕ) (x : ℕ) : Expr -> Expr
   | .plus₂ l r => .plus₂ (closing i x l) (closing i x r)
   | .code e => .code (closing i x e)
   | .reflect e => .reflect (closing i x e)
-  | .lam𝕔 τ e => .lam𝕔 τ (closing (i + 1) x e)
+  | .lam𝕔 e => .lam𝕔 (closing (i + 1) x e)
   | .lets b e => .lets (closing i x b) (closing (i + 1) x e)
   | .let𝕔 b e => .let𝕔 (closing i x b) (closing (i + 1) x e)
 
@@ -115,8 +115,8 @@ def closed_at (e : Expr) (f : ℕ) : Prop :=
   match e with
   | .bvar _ => true
   | .fvar x => x < f
-  | .lam₁ _ e => closed_at e f
-  | .lam₂ _ e => closed_at e f
+  | .lam₁ e => closed_at e f
+  | .lam₂ e => closed_at e f
   | .app₁ e1 e2 => closed_at e1 f ∧ closed_at e2 f
   | .app₂ e1 e2 => closed_at e1 f ∧ closed_at e2 f
   | .lit₁ _ => true
@@ -125,7 +125,7 @@ def closed_at (e : Expr) (f : ℕ) : Prop :=
   | .plus₂ l r => closed_at l f ∧ closed_at r f
   | .code e => closed_at e f
   | .reflect e => closed_at e f
-  | .lam𝕔 _ e => closed_at e f
+  | .lam𝕔 e => closed_at e f
   | .lets b e => closed_at b f ∧ closed_at e f
   | .let𝕔 b e => closed_at b f ∧ closed_at e f
 
@@ -135,8 +135,8 @@ def closedb_at (e : Expr) (b : ℕ) : Prop :=
   match e with
   | .bvar x => x < b
   | .fvar _ => true
-  | .lam₁ _ e => closedb_at e (b + 1)
-  | .lam₂ _ e => closedb_at e (b + 1)
+  | .lam₁ e => closedb_at e (b + 1)
+  | .lam₂ e => closedb_at e (b + 1)
   | .app₁ e1 e2 => closedb_at e1 b ∧ closedb_at e2 b
   | .app₂ e1 e2 => closedb_at e1 b ∧ closedb_at e2 b
   | .lit₁ _ => true
@@ -145,7 +145,7 @@ def closedb_at (e : Expr) (b : ℕ) : Prop :=
   | .plus₂ l r => closedb_at l b ∧ closedb_at r b
   | .code e => closedb_at e b
   | .reflect e => closedb_at e b
-  | .lam𝕔 _ e => closedb_at e (b + 1)
+  | .lam𝕔 e => closedb_at e (b + 1)
   | .lets e1 e2 => closedb_at e1 b ∧ closedb_at e2 (b + 1)
   | .let𝕔 e1 e2 => closedb_at e1 b ∧ closedb_at e2 (b + 1)
 
@@ -175,9 +175,9 @@ lemma subst_closed_id : ∀ x e v, closed_at e x -> subst x v e = e :=
   induction e with
   | bvar => simp
   | fvar => simp at *; omega
-  | lam₁ _ _ IH
-  | lam₂ _ _ IH
-  | lam𝕔 _ _ IH =>
+  | lam₁ _ IH
+  | lam₂ _ IH
+  | lam𝕔 _ IH =>
     simp; apply IH; apply He
   | app₁ _ _ IH₀ IH₁
   | app₂ _ _ IH₀ IH₁
@@ -239,9 +239,9 @@ lemma closed_inc : ∀ x y e, closed_at e x -> x <= y -> closed_at e y :=
     apply IH₀; apply Hclose.left
     apply IH₁; apply Hclose.right
   | lit₁| lit₂ => simp
-  | lam₁ _ _ IH
-  | lam₂ _ _ IH
-  | lam𝕔 _ _ IH
+  | lam₁ _ IH
+  | lam₂ _ IH
+  | lam𝕔 _ IH
   | code _ IH
   | reflect _ IH =>
     simp; apply IH; apply Hclose
@@ -255,9 +255,9 @@ lemma subst_closedb_at : ∀ x e v i, closedb_at v i -> closedb_at e i -> closed
     by_cases HEq : x = y
     . rw [HEq]; simp; apply Hv
     . simp; rw [if_neg HEq]; simp
-  | lam₁ _ _ IH
-  | lam₂ _ _ IH
-  | lam𝕔 _ _ IH =>
+  | lam₁ _ IH
+  | lam₂ _ IH
+  | lam𝕔 _ IH =>
     apply IH; apply closedb_inc; apply Hv; omega; apply He
   | app₁ _ _ IH₀ IH₁
   | app₂ _ _ IH₀ IH₁
@@ -285,9 +285,9 @@ lemma subst_closed_at : ∀ x e v y, closed_at v y -> closed_at e y -> closed_at
     by_cases HEq : x = z
     . rw [HEq]; simp; apply Hv
     . simp; rw [if_neg HEq]; apply He
-  | lam₁ _ _ IH
-  | lam₂ _ _ IH
-  | lam𝕔 _ _ IH =>
+  | lam₁ _ IH
+  | lam₂ _ IH
+  | lam𝕔 _ IH =>
     apply IH; apply Hv; apply He
   | app₁ _ _ IH₀ IH₁
   | app₂ _ _ IH₀ IH₁
@@ -312,9 +312,9 @@ lemma subst_closed_at_dec : ∀ x e v, closed_at v x -> closed_at e (x + 1) -> c
     by_cases HEq : x = z
     . rw [← HEq]; simp; apply Hv
     . simp; rw [if_neg HEq]; simp at *; omega
-  | lam₁ _ _ IH
-  | lam₂ _ _ IH
-  | lam𝕔 _ _ IH =>
+  | lam₁ _ IH
+  | lam₂ _ IH
+  | lam𝕔 _ IH =>
     apply IH; apply He
   | app₁ _ _ IH₀ IH₁
   | app₂ _ _ IH₀ IH₁
@@ -388,9 +388,9 @@ theorem close_closed : ∀ e x i, closed_at e (x + 1) → closed_at (closing i x
     . rw [HEq]; simp
     . simp; rw [if_neg HEq]; simp; omega
   | bvar => simp
-  | lam₁ _ _ IH
-  | lam₂ _ _ IH
-  | lam𝕔 _ _ IH
+  | lam₁ _ IH
+  | lam₂ _ IH
+  | lam𝕔 _ IH
   | code _ IH
   | reflect _ IH => apply IH
   | app₁ _ _ IH₀ IH₁
@@ -413,9 +413,9 @@ theorem open_closed : ∀ e x i, closed_at e x → closed_at (opening i (.fvar x
     by_cases HEq : j = i
     . rw [HEq]; simp
     . simp; rw [if_neg HEq]; simp
-  | lam₁ _ _ IH
-  | lam₂ _ _ IH
-  | lam𝕔 _ _ IH
+  | lam₁ _ IH
+  | lam₂ _ IH
+  | lam𝕔 _ IH
   | code _ IH
   | reflect _ IH => apply IH
   | app₁ _ _ IH₀ IH₁
@@ -438,9 +438,9 @@ theorem close_closedb : ∀ e x i j, j < i -> closedb_at e i → closedb_at (clo
     . rw [HEq]; simp; omega
     . simp; rw [if_neg HEq]; simp
   | bvar => simp
-  | lam₁ _ _ IH
-  | lam₂ _ _ IH
-  | lam𝕔 _ _ IH
+  | lam₁ _ IH
+  | lam₂ _ IH
+  | lam𝕔 _ IH
   | code _ IH
   | reflect _ IH =>
     apply IH; omega
@@ -488,9 +488,9 @@ lemma open_close_id : ∀ i e x, closedb_at e i -> opening i (.fvar x) (closing 
     by_cases HEq : x = y
     . rw [HEq]; simp
     . rw [if_neg HEq]; simp
-  | lam₁ _ _ IHe
-  | lam₂ _ _ IHe
-  | lam𝕔 _ _ IHe
+  | lam₁ _ IHe
+  | lam₂ _ IHe
+  | lam𝕔 _ IHe
   | code _ IHe
   | reflect _ IHe =>
     simp; apply IHe; apply Hlc
@@ -536,9 +536,9 @@ lemma subst_opening_comm :
   | reflect _ IH =>
     simp; apply IH; apply Hclosedb
   | lit₁| lit₂ => simp
-  | lam₁ _ _ IH
-  | lam₂ _ _ IH
-  | lam𝕔 _ _ IH =>
+  | lam₁ _ IH
+  | lam₂ _ IH
+  | lam𝕔 _ IH =>
     simp; apply IH; apply closedb_inc; apply Hclosedb; omega
 
 lemma subst_open₀_comm : ∀ x y e v, x ≠ y -> lc v -> subst x v (open₀ y e) = open₀ y (subst x v e) := by
@@ -549,8 +549,8 @@ def maping𝕔 (e : Expr) (i : ℕ) : Expr :=
   match e with
   | .bvar j => if j == i then (.code (.bvar i)) else .bvar j
   | .fvar x => .fvar x
-  | .lam₁ τ e => .lam₁ τ (maping𝕔 e (i + 1))
-  | .lam₂ τ e => .lam₂ τ (maping𝕔 e (i + 1))
+  | .lam₁ e => .lam₁ (maping𝕔 e (i + 1))
+  | .lam₂ e => .lam₂ (maping𝕔 e (i + 1))
   | .app₁ f arg => .app₁ (maping𝕔 f i) (maping𝕔 arg i)
   | .app₂ f arg => .app₂ (maping𝕔 f i) (maping𝕔 arg i)
   | .lit₁ n => .lit₁ n
@@ -559,12 +559,12 @@ def maping𝕔 (e : Expr) (i : ℕ) : Expr :=
   | .plus₂ l r => .plus₂ (maping𝕔 l i) (maping𝕔 r i)
   | .code e => .code (maping𝕔 e i)
   | .reflect e => .reflect (maping𝕔 e i)
-  | .lam𝕔 τ e => .lam𝕔 τ (maping𝕔 e (i + 1))
+  | .lam𝕔 e => .lam𝕔 (maping𝕔 e (i + 1))
   | .lets b e => .lets (maping𝕔 b i) (maping𝕔 e (i + 1))
   | .let𝕔 b e => .let𝕔 (maping𝕔 b i) (maping𝕔 e (i + 1))
 
 inductive value : Expr -> Prop where
-  | lam₁ : ∀ e, lc (.lam₁ _ e) -> value (.lam₁ _ e)
+  | lam₁ : ∀ e, lc (.lam₁ e) -> value (.lam₁ e)
   | lit₁ : ∀ n, value (.lit₁ n)
   | code : ∀ e, lc e -> value (.code e)
 
@@ -579,7 +579,7 @@ theorem value_lc : ∀ e, value e -> lc e := by
 def map𝕔₀ (e : Expr) : Expr :=
   maping𝕔 e 0
 
-example : map𝕔₀ (.app₁ (.bvar 0) (.lam₁ .nat (.bvar 1))) = .app₁ (.code (.bvar 0)) (.lam₁ .nat (.code (.bvar 1))) := by simp
+example : map𝕔₀ (.app₁ (.bvar 0) (.lam₁ (.bvar 1))) = .app₁ (.code (.bvar 0)) (.lam₁ (.code (.bvar 1))) := by simp
 
 theorem maping𝕔_intro :
     ∀ x e i, closed_at e x -> closing i x (subst x (.code (.fvar x)) (opening i (.fvar x) e)) = maping𝕔 e i :=
@@ -588,11 +588,11 @@ theorem maping𝕔_intro :
   induction e generalizing i with
   | bvar j => by_cases HEq : j = i; rw [HEq]; simp; simp [if_neg HEq]
   | fvar y => simp at *; by_cases HEq : x = y; omega; rw [if_neg HEq]; simp; apply HEq
-  | lam₁ _ _ ih
-  | lam₂ _ _ ih
+  | lam₁ _ ih
+  | lam₂ _ ih
   | code _ ih
   | reflect _ ih
-  | lam𝕔 _ _ ih =>
+  | lam𝕔 _ ih =>
     simp at *; apply ih; apply Hclosed
   | app₁ _ _ ih1 ih2
   | app₂ _ _ ih1 ih2
@@ -614,8 +614,8 @@ theorem map𝕔₀_intro : ∀ x e, closed_at e x -> close₀ x (subst x (.code 
 def shiftl_at (x : ℕ) (n : ℕ) : Expr -> Expr
   | .bvar i => .bvar i
   | .fvar y => if x <= y then .fvar (y + n) else .fvar y
-  | .lam₁ τ e => .lam₁ τ (shiftl_at x n e)
-  | .lam₂ τ e => .lam₂ τ (shiftl_at x n e)
+  | .lam₁ e => .lam₁ (shiftl_at x n e)
+  | .lam₂ e => .lam₂ (shiftl_at x n e)
   | .app₁ f arg => .app₁ (shiftl_at x n f) (shiftl_at x n arg)
   | .app₂ f arg => .app₂ (shiftl_at x n f) (shiftl_at x n arg)
   | .lit₁ n => .lit₁ n
@@ -624,7 +624,7 @@ def shiftl_at (x : ℕ) (n : ℕ) : Expr -> Expr
   | .plus₂ l r => .plus₂ (shiftl_at x n l) (shiftl_at x n r)
   | .code e => .code (shiftl_at x n e)
   | .reflect e => .reflect (shiftl_at x n e)
-  | .lam𝕔 τ e => .lam𝕔 τ (shiftl_at x n e)
+  | .lam𝕔 e => .lam𝕔 (shiftl_at x n e)
   | .lets b e => .lets (shiftl_at x n b) (shiftl_at x n e)
   | .let𝕔 b e => .let𝕔 (shiftl_at x n b) (shiftl_at x n e)
 
@@ -649,9 +649,9 @@ theorem shiftl_opening :
   | let𝕔 _ _ IH₀ IH₁ =>
     simp; constructor; apply IH₀; apply IH₁
   | lit₁| lit₂ => simp
-  | lam₁ _ _ IH
-  | lam₂ _ _ IH
-  | lam𝕔 _ _ IH
+  | lam₁ _ IH
+  | lam₂ _ IH
+  | lam𝕔 _ IH
   | code _ IH
   | reflect _ IH =>
     simp; apply IH
@@ -679,9 +679,9 @@ theorem shiftl_closed_at :
     apply IH₀; apply Hclose.left
     apply IH₁; apply Hclose.right
   | lit₁| lit₂ => simp
-  | lam₁ _ _ IH
-  | lam₂ _ _ IH
-  | lam𝕔 _ _ IH
+  | lam₁ _ IH
+  | lam₂ _ IH
+  | lam𝕔 _ IH
   | code _ IH
   | reflect _ IH =>
     simp; apply IH; apply Hclose
@@ -703,9 +703,9 @@ theorem shiftl_id :
     apply IH₀; apply Hclose.left
     apply IH₁; apply Hclose.right
   | lit₁| lit₂ => simp
-  | lam₁ _ _ IH
-  | lam₂ _ _ IH
-  | lam𝕔 _ _ IH
+  | lam₁ _ IH
+  | lam₂ _ IH
+  | lam𝕔 _ IH
   | code _ IH
   | reflect _ IH =>
     simp; apply IH
@@ -714,8 +714,8 @@ theorem shiftl_id :
 def shiftr_at (x : ℕ) : Expr -> Expr
   | .bvar i => .bvar i
   | .fvar y => if x < y then .fvar (y - 1) else .fvar y
-  | .lam₁ τ e => .lam₁ τ (shiftr_at x e)
-  | .lam₂ τ e => .lam₂ τ (shiftr_at x e)
+  | .lam₁ e => .lam₁ (shiftr_at x e)
+  | .lam₂ e => .lam₂ (shiftr_at x e)
   | .app₁ f arg => .app₁ (shiftr_at x f) (shiftr_at x arg)
   | .app₂ f arg => .app₂ (shiftr_at x f) (shiftr_at x arg)
   | .lit₁ n => .lit₁ n
@@ -724,7 +724,7 @@ def shiftr_at (x : ℕ) : Expr -> Expr
   | .plus₂ l r => .plus₂ (shiftr_at x l) (shiftr_at x r)
   | .code e => .code (shiftr_at x e)
   | .reflect e => .reflect (shiftr_at x e)
-  | .lam𝕔 τ e => .lam𝕔 τ (shiftr_at x e)
+  | .lam𝕔 e => .lam𝕔 (shiftr_at x e)
   | .lets b e => .lets (shiftr_at x b) (shiftr_at x e)
   | .let𝕔 b e => .let𝕔 (shiftr_at x b) (shiftr_at x e)
 
@@ -749,9 +749,9 @@ theorem shiftr_opening :
   | let𝕔 _ _ IH₀ IH₁ =>
     simp; constructor; apply IH₀; apply IH₁
   | lit₁| lit₂ => simp
-  | lam₁ _ _ IH
-  | lam₂ _ _ IH
-  | lam𝕔 _ _ IH
+  | lam₁ _ IH
+  | lam₂ _ IH
+  | lam𝕔 _ IH
   | code _ IH
   | reflect _ IH =>
     simp; apply IH
@@ -780,9 +780,9 @@ theorem shiftr_closed_at : ∀ x y e, y < x -> closed_at e (x + 1) -> closed_at 
     apply IH₀; apply Hclose.left
     apply IH₁; apply Hclose.right
   | lit₁| lit₂ => simp
-  | lam₁ _ _ IH
-  | lam₂ _ _ IH
-  | lam𝕔 _ _ IH
+  | lam₁ _ IH
+  | lam₂ _ IH
+  | lam𝕔 _ IH
   | code _ IH
   | reflect _ IH =>
     simp; apply IH; apply Hclose
@@ -806,9 +806,9 @@ theorem shiftr_closed_at_id : ∀ x e, closed_at e x -> closed_at (shiftr_at x e
     apply IH₀; apply Hclose.left
     apply IH₁; apply Hclose.right
   | lit₁| lit₂ => simp
-  | lam₁ _ _ IH
-  | lam₂ _ _ IH
-  | lam𝕔 _ _ IH
+  | lam₁ _ IH
+  | lam₂ _ IH
+  | lam𝕔 _ IH
   | code _ IH
   | reflect _ IH =>
     simp; apply IH; apply Hclose
@@ -830,9 +830,9 @@ theorem shiftr_id :
     apply IH₀; apply Hclose.left
     apply IH₁; apply Hclose.right
   | lit₁| lit₂ => simp
-  | lam₁ _ _ IH
-  | lam₂ _ _ IH
-  | lam𝕔 _ _ IH
+  | lam₁ _ IH
+  | lam₂ _ IH
+  | lam𝕔 _ IH
   | code _ IH
   | reflect _ IH =>
     simp; apply IH
